% For double-blind review submission, w/o CCS and ACM Reference (max
% submission space)
\documentclass[acmsmall,review,anonymous]{acmart}
\settopmatter{printfolios=true,printccs=false,printacmref=false}
%% For double-blind review submission, w/ CCS and ACM Reference
%\documentclass[acmsmall,review,anonymous]{acmart}\settopmatter{printfolios=true}
%% For single-blind review submission, w/o CCS and ACM Reference (max submission space)
%\documentclass[acmsmall,review]{acmart}\settopmatter{printfolios=true,printccs=false,printacmref=false}
%% For single-blind review submission, w/ CCS and ACM Reference
%\documentclass[acmsmall,review]{acmart}\settopmatter{printfolios=true}
%% For final camera-ready submission, w/ required CCS and ACM Reference
%\documentclass[acmsmall]{acmart}\settopmatter{}


%% Journal information
%% Supplied to authors by publisher for camera-ready submission;
%% use defaults for review submission.
\acmJournal{PACMPL}
\acmVolume{1}
\acmNumber{POPL} % CONF = POPL or ICFP or OOPSLA
\acmArticle{1}
\acmYear{2020}
\acmMonth{1}
\acmDOI{} % \acmDOI{10.1145/nnnnnnn.nnnnnnn}
\startPage{1}

%% Copyright information
%% Supplied to authors (based on authors' rights management selection;
%% see authors.acm.org) by publisher for camera-ready submission;
%% use 'none' for review submission.
\setcopyright{none}
%\setcopyright{acmcopyright}
%\setcopyright{acmlicensed}
%\setcopyright{rightsretained}
%\copyrightyear{2018}           %% If different from \acmYear

%% Bibliography style
\bibliographystyle{ACM-Reference-Format}
%% Citation style
%% Note: author/year citations are required for papers published as an
%% issue of PACMPL.
\citestyle{acmauthoryear}   %% For author/year citations
%\citestyle{acmnumeric}

%%%%%%%%%%%%%%%%%%%%%%%%%%%%%%%%%%%%%%%%%%%%%%%%%%%%%%%%%%%%%%%%%%%%%%
%% Note: Authors migrating a paper from PACMPL format to traditional
%% SIGPLAN proceedings format must update the '\documentclass' and
%% topmatter commands above; see 'acmart-sigplanproc-template.tex'.
%%%%%%%%%%%%%%%%%%%%%%%%%%%%%%%%%%%%%%%%%%%%%%%%%%%%%%%%%%%%%%%%%%%%%%



\usepackage[utf8]{inputenc}
\usepackage{ccicons}

\usepackage{amsmath}
\usepackage{amsthm}
\usepackage{amscd}
%\usepackage{MnSymbol}
\usepackage{xcolor}

\usepackage{bbold}
\usepackage{url}
\usepackage{upgreek}
%\usepackage{stmaryrd}

\usepackage{lipsum}
\usepackage{tikz-cd}
\usetikzlibrary{cd}
\usetikzlibrary{calc}
\usetikzlibrary{arrows}

\usepackage{bussproofs}
\EnableBpAbbreviations

\input{macros}
\input{mytheorem}

\theoremstyle{definition}
\newtheorem{exmpl}{Example}

\renewcommand{\greyout}[1]{} %{{\color{gray} {#1}}} -- toggle to remove greyed text

\newcommand{\emptyfun}{{[]}}
\newcommand{\cal}{\mathcal}
%\newcommand{\fold}{\mathit{fold}}
\newcommand{\F}{\mathcal{F}}
\renewcommand{\G}{\mathcal{G}}
\newcommand{\N}{\mathcal{N}}
\newcommand{\E}{\mathcal{E}}
\newcommand{\B}{\mathcal{B}}
\renewcommand{\P}{\mathcal{A}}
\newcommand{\pred}{\mathsf{Fam}}
\newcommand{\env}{\mathsf{Env}}
\newcommand{\set}{\mathsf{Set}}
\renewcommand{\S}{\mathcal S}
\renewcommand{\C}{\mathcal{C}}
\newcommand{\D}{\mathcal{D}}
\newcommand{\A}{\mathcal{A}}
\renewcommand{\id}{\mathit{id}}
\newcommand{\map}{\mathsf{map}}
\newcommand{\pid}{\underline{\mathit{id}}}
\newcommand{\pcirc}{\,\underline{\circ}\,}
\newcommand{\pzero}{\underline{0}}
\newcommand{\pone}{\underline{1}}
\newcommand{\psum}{\,\underline{+}\,}
%\newcommand{\inl}{\mathit{inL}\,}
%\newcommand{\inr}{\mathit{inR}\,}
\newcommand{\pinl}{\underline{\mathit{inL}}\,}
\newcommand{\pinr}{\underline{\mathit{inR}}\,}
\newcommand{\ptimes}{\,\underline{\times}\,}
\newcommand{\ppi}{\underline{\pi_1}}
\newcommand{\pppi}{\underline{\pi_2}}
\newcommand{\pmu}{\underline{\mu}}

\title[Free Theorems for Nested Types]{Free Theorems for 
Nested Types} %% [Short Title] is optional;
                                        %% when present, will be used in
                                        %% header instead of Full Title.
%\titlenote{with title note}             %% \titlenote is optional;
                                        %% can be repeated if necessary;
                                        %% contents suppressed with 'anonymous'
%\subtitle{Subtitle}                     %% \subtitle is optional
%\subtitlenote{with subtitle note}       %% \subtitlenote is optional;
                                        %% can be repeated if necessary;
                                        %% contents suppressed with 'anonymous'

\begin{document}
\maketitle
\section{Demotion Theorems}

\begin{thm}

If $\Gamma; \Phi, \phi^k \vdash \tau : \F$, then one can derive
$\Gamma, \psi^k; \Phi \vdash \tau[\phi^k :== \psi^k]$, 
where $\tau[\phi :== \psi]$ is the textual replacement of $\phi$ in $\tau$.
In other words, all occurences of $\phi\ol\sigma$ in $\tau$ become $\psi\ol\sigma$.
\end{thm}
\begin{proof}
By induction on the structure of $\tau$.
\begin{itemize}
  \item There is nothing to prove for types in $\T$ because their functorial contexts
        must be empty.
  \item Case $\Gamma; \Phi, \alpha \vdash \alpha : \F$. We must
    derive $\Gamma, \beta; \Phi \vdash \beta : \F$. 
    
    \[\begin{array}{c}
    \AXC{$\Gamma, \beta; \emptyset \vdash \beta : \T$}
    \UIC{$\Gamma, \beta; \emptyset \vdash \beta : \F$}
    \UIC{$\Gamma, \beta; \Phi   \vdash \beta : \F$}
    \DP
    \end{array}\]  \\

  \item Case $\Gamma; \Phi, \phi \vdash \onet :\F$,  $\Gamma; \Phi, \phi \vdash \zerot :\F$.
        We can immediately form the required judgments. \\

  \item Case $\Gamma; \Phi, \phi \vdash \phi \ol\tau : \F$. We must derive 
    $\Gamma, \psi; \Phi \vdash (\phi \ol\tau) [\phi :== \psi] : \F$. The induction hypothesis 
    gives that $\Gamma, \psi; \Phi \vdash \tau[\phi :== \psi] : \F$ for each $\tau$. 

    \[\begin{array}{c}
    \AXC{$\psi \in \{ \Gamma, \psi \} \cup \Phi : \F$}
      \AXC{$\ol{\Gamma, \psi; \Phi \vdash \tau[\phi :== \psi] : \F}$}
      \BIC{$\Gamma, \psi; \Phi \vdash \psi \ol{\tau[\phi :== \psi]} : \F$}
    \UIC{$\Gamma, \psi; \Phi \vdash (\phi \ol\tau)[\phi :== \psi] :\F$}
    \DP
    \end{array}\]  

    The case for $\Gamma; \Phi, \phi' \vdash \phi \ol\tau : \F$, i.e., the case in which
    the variable being ``demoted'' only appears in the arguments, 
    works by the same induction. \\

  \item Case $\Gamma; \Phi, \phi \vdash (\mu \phi'. \lambda \ol\alpha. H)\ol\tau : \F$. 
    We must derive $\Gamma, \psi; \Phi \vdash ((\mu \phi'. \lambda \ol\alpha. H)
     \ol\tau)[\phi :== \psi] : \F$. The induction hypothesis gives that 
     $\Gamma, \psi; \Phi \vdash \tau[\phi :== \psi] : \F$ for each $\tau$ and
     $\Gamma, \psi; \Phi, \ol\alpha, \phi' \vdash H[\phi :== \psi] : \F$.

    \[\begin{array}{c}
      \AXC{$\Gamma, \psi; \Phi, \ol\alpha, \phi' \vdash H[\phi :== \psi] : \F$}
      \AXC{$\ol{\Gamma, \psi; \Phi \vdash \tau[\phi :== \psi] : \F}$}
      \BIC{$\Gamma, \psi; \Phi \vdash (\mu \phi'. \lambda \ol\alpha. H[\phi :== \psi])
        \ol{\tau[\phi :== \psi]} : \F$}
      \UIC{$\Gamma, \psi; \Phi \vdash ((\mu \phi'. \lambda \ol\alpha. H)\ol\tau)[\phi :== \psi] : \F$}
    \DP
    \end{array}\]  \\

  \item Case $\Gamma; \Phi, \phi \vdash \sigma \times \tau : \F$. We must derive
    $\Gamma, \psi; \Phi \vdash (\sigma \times \tau) [\phi :== \psi] : \F$. 
    The induction hypothesis gives that
    $\Gamma, \psi; \Phi \vdash \sigma [\phi :== \psi]: \F$ and
    $\Gamma, \psi; \Phi \vdash \tau [\phi :== \psi]: \F$. 

    \[\begin{array}{c}
      \AXC{$\Gamma, \psi; \Phi \vdash \sigma [\phi :== \psi]: \F$}
      \AXC{$\Gamma, \psi; \Phi \vdash \tau   [\phi :== \psi]: \F$}
      \BIC{$\Gamma, \psi; \Phi \vdash \sigma [\phi :== \psi] \times \tau [\phi :== \psi]: \F$}
      \UIC{$\Gamma, \psi; \Phi \vdash (\sigma \times \tau) [\phi :== \psi]: \F$}
    \DP
    \end{array}\]  

  The case for $\sigma + \tau$ is analogous.

\end{itemize}

\end{proof}

      % $$
      % \setsem{\Gamma; \Phi, \phi \vdash ____ : \F} \rho = 
      % $$

Note that the next two theorems are proven by 
simultaneous induction. We are actually only interested in using Theorem~\ref{thm:demotion-objects}, 
but in order to prove the $\mu$ case for this theorem, we need Theorem~\ref{thm:demotion-morph} 
to show that two functors have equal actions on morphisms.


\begin{thm}\label{thm:demotion-objects}
If $\Gamma; \Phi, \phi \vdash  \tau : \F$, $\rho : \setenv$, and $\rho \phi = \rho \psi$, then
  $$\setsem{\Gamma; \Phi, \phi \vdash \tau} \rho = \setsem{\Gamma, \psi; \Phi \vdash \tau[\phi :== \psi] } \rho $$

Analogously, if $\rho :\relenv$, and $\rho \phi = \rho \psi$, then
$$\relsem{\Gamma; \Phi, \phi \vdash \tau} \rho = \relsem{\Gamma, \psi; \Phi \vdash \tau[\phi :== \psi] } \rho $$

\end{thm}
\begin{proof}
We prove the case for $\set$ by induction on the structure of $\tau$.
The case for $\rel$ proceeds analogously.
\begin{itemize}
  \item There is nothing to prove for types in $\T$ because their functorial contexts
        must be empty.
  \item Case $\Gamma; \Phi, \alpha \vdash \alpha : \F$. Given that $\rho \alpha = \rho \beta$, 
    \begin{align*}
         & \setsem{\Gamma; \Phi, \alpha \vdash \alpha } \rho \\
    = \; & \rho \alpha \\
    = \; & \rho \beta \\
    = \; & \setsem{\Gamma, \beta; \Phi \vdash \beta } \rho
    \end{align*}

  \item Case $\Gamma; \Phi, \phi \vdash \onet :\F$,  $\Gamma; \Phi, \phi \vdash \zerot :\F$.
    \begin{align*}
         & \setsem{\Gamma; \Phi, \phi \vdash \onet } \rho \\
    = \; & 1 \\
    = \; & \setsem{\Gamma, \psi; \Phi \vdash \onet } \rho
    \end{align*}

    Similarly for $\zerot$.

  \item Case $\Gamma; \Phi, \phi \vdash \phi \ol\tau : \F$. The induction hypothesis gives that 
    $$\setsem{\Gamma; \Phi, \phi \vdash \tau } \rho
      = \setsem{\Gamma, \psi; \Phi \vdash \tau[\phi :== \psi] } \rho$$ 
    for each $\tau$.
    \begin{align*}
         & \setsem{\Gamma; \Phi, \phi \vdash \phi \ol\tau } \rho \\
      = \; & (\rho \phi) \ol{\setsem{\Gamma; \Phi, \phi \vdash \tau } \rho} \\
      = \; & (\rho \phi) \ol{\setsem{\Gamma, \psi; \Phi \vdash \tau[\phi :== \psi] } \rho} \\
      = \; & (\rho \psi) \ol{\setsem{\Gamma, \psi; \Phi \vdash \tau[\phi :== \psi] } \rho} \\
      = \; & \setsem{\Gamma, \psi; \Phi \vdash \psi \ol{\tau[\phi :== \psi]} } \rho \\
      = \; & \setsem{\Gamma, \psi; \Phi \vdash (\phi \ol\tau)[\phi :== \psi] } \rho
    \end{align*}
  
    The first and fifth equalities above are by Definition~\ref{def:set-sem}. The fourth equality
    is by equality of the functors $\rho \phi$ and $\rho \psi$.  \\

  \item Case $\Gamma; \Phi, \phi \vdash (\mu \phi'. \lambda \ol\alpha. H)\ol\tau : \F$. 
      The induction hypothesis gives that 
      $$\setsem{\Gamma; \Phi, \phi', \ol{\alpha}, \phi \vdash H } \rho
        = \setsem{\Gamma, \psi; \Phi, \phi', \ol{\alpha} \vdash H[\phi :== \psi] } \rho$$ 
      and 
      $$\setsem{\Gamma; \Phi, \phi \vdash \tau } \rho
        = \setsem{\Gamma, \psi; \Phi \vdash \tau[\phi :== \psi] } \rho$$ 
      for each $\tau$. 

      \begin{align*}
        & \setsem{\Gamma; \Phi, \phi \vdash (\mu \phi'. \lambda \ol\alpha. H)\ol\tau } \rho \\
        %% = \; & (\mu T_{\rho}^\set) \ol{\setsem{ \Gamma; \Phi, \phi \vdash \tau} \rho} \text{\quad(T contains $\phi$)} \\ 
        % = \; & (\mu T_{\rho}^\set) \ol{\setsem{ \Gamma; \Phi, \phi \vdash \tau} \rho} \text{\quad(T contains $\phi$)} \\ 
        = \; & (\mu (
            \lambda F. \lambda \ol{A}. \setsem{\Gamma; \Phi, \phi', \ol{\alpha}, \phi \vdash H} \rho[\phi' := F][\ol{\alpha := A}]
          )
        ) \ol{\setsem{ \Gamma; \Phi, \phi \vdash \tau} \rho} \\
        = \; & (\mu (
            \lambda F. \lambda \ol{A}. \setsem{\Gamma, \psi; \Phi, \phi', \ol{\alpha} \vdash H[\phi :== \psi]} \rho[\phi' := F][\ol{\alpha := A}]
          )
        ) \ol{\setsem{ \Gamma; \Phi, \phi \vdash \tau} \rho} \\
        % = \; &  (\mu (
        %     \lambda F. \lambda \ol{A}. \setsem{\Gamma, \psi; \Phi, \phi', \ol{\alpha} \vdash H[\phi :== \psi]} \rho[\phi' := F][\ol{\alpha := A}]
        %   ) \ol{\setsem{ \Gamma; \Phi, \phi \vdash \tau} \rho} \\
        = \; &  (\mu (
            \lambda F. \lambda \ol{A}. \setsem{\Gamma, \psi; \Phi, \phi', \ol{\alpha} \vdash H[\phi :== \psi]} \rho[\phi' := F][\ol{\alpha := A}]
          )
        \ol{\setsem{ \Gamma, \psi; \Phi \vdash \tau[\phi :== \psi]} \rho} \\
        = \; & \setsem{\Gamma, \psi; \Phi \vdash (\mu \phi'. \lambda \ol\alpha. H[\phi :== \psi]) \ol{\tau[\phi :== \psi]} } \rho \\
        = \; & \setsem{\Gamma, \psi; \Phi \vdash ((\mu \phi'. \lambda \ol\alpha. H) \ol\tau)[\phi :== \psi] } \rho 
      \end{align*} 
      The first and fifth equalities are by Definition~\ref{def:set-sem}.
      The second equality follows from the following equality:
      \begin{align*}
        &\lambda F. \lambda \ol{A}. \setsem{\Gamma; \Phi, \phi', \ol{\alpha}, \phi \vdash H} \rho[\phi' := F][\ol{\alpha := A}] \\
        & = \lambda F. \lambda \ol{A}. \setsem{\Gamma, \psi; \Phi, \phi', \ol{\alpha} \vdash H[\phi :== \psi]} \rho[\phi' := F][\ol{\alpha := A}]
      \end{align*}
      These two functors have the same action on objects by the induction hypothesis on $H$, and the fact
      that the extended environment $\rho[\phi' := F][\ol{\alpha := A}]$ satisfies the required
      hypothesis. These two functors have the same action on morphisms by the induction hypothesis
      on $H$ from Theorem~\ref{thm:demotion-morph}. Thus they are the same functor with the same fixed point.

  \item Case $\Gamma; \Phi, \phi \vdash \sigma \times \tau : \F$. The induction hypothesis gives that 
      $$\setsem{\Gamma; \Phi, \phi \vdash \sigma } \rho
        = \setsem{\Gamma, \psi; \Phi \vdash \sigma[\phi :== \psi] } \rho$$ 
        and
      $$\setsem{\Gamma; \Phi, \phi \vdash \tau } \rho
        = \setsem{\Gamma, \psi; \Phi \vdash \tau[\phi :== \psi] } \rho$$ 

    \begin{align*}
           & \setsem{\Gamma; \Phi, \phi \vdash \sigma \times \tau} \rho \\
      = \; & \setsem{\Gamma; \Phi, \phi \vdash \sigma} \rho \times \setsem{\Gamma; \Phi, \phi \vdash \tau} \rho\\
      = \; & \setsem{\Gamma, \psi; \Phi \vdash \sigma[\phi :== \psi]} \rho \times \setsem{\Gamma, \psi; \Phi \vdash \tau[\phi :== \psi]} \rho\\
      = \; & \setsem{\Gamma, \psi; \Phi \vdash \sigma[\phi :==\psi] \times \tau[\phi :== \psi]} \rho \\
      = \; & \setsem{\Gamma, \psi; \Phi \vdash (\sigma \times \tau)[\phi :== \psi]} \rho
    \end{align*}

    The case for $\sigma + \tau$ is analogous.
\end{itemize}
\end{proof}

\begin{thm}\label{thm:demotion-morph}
If $\Gamma; \Phi, \phi \vdash \tau : \F$, and if 
$f : \rho \to \rho'$, is a morphism of set environments such that
  $\rho \phi = \rho \psi = \rho' \phi = \rho' \psi$, and
   $f \phi = f \psi = \id_{\rho \phi}$, then

  $$\setsem{\Gamma; \Phi, \phi \vdash \tau} f 
    = \setsem{\Gamma, \psi; \Phi \vdash \tau[\phi :== \psi]} f $$

Analogously, if
$f : \rho \to \rho'$, is a morphism of relation environments such that
  $\rho \phi = \rho \psi = \rho' \phi = \rho' \psi$, and
   $f \phi = f \psi = \id_{\rho \phi}$, then

  $$\relsem{\Gamma; \Phi, \phi \vdash \tau} f 
    = \relsem{\Gamma, \psi; \Phi \vdash \tau[\phi :== \psi]} f $$

\end{thm}

\begin{proof}
We prove the case for $\set$ by induction on the structure of $\tau$.
The case for $\rel$ proceeds analogously.

\begin{itemize}
  \item There is nothing to prove for types in $\T$ because their functorial contexts
        must be empty.
  \item Case $\Gamma; \Phi, \alpha \vdash \alpha : \F$. Given that $\rho \alpha = \rho \beta$, 
      
    \begin{align*}
         & \setsem{\Gamma; \Phi, \alpha \vdash \alpha } f \\
      = \; & \id_{\rho \alpha} \\
      = \; & \id_{\rho \beta}  \\
      = \; & \setsem{\Gamma, \beta; \Phi \vdash \beta } f
    \end{align*}

  \item Case $\Gamma; \Phi, \phi \vdash \onet :\F$,  $\Gamma; \Phi, \phi \vdash \zerot :\F$.

    \begin{align*}
         & \setsem{\Gamma; \Phi, \phi \vdash \onet } f \\
      = \; & \id_1 \\
      = \; & \setsem{\Gamma, \psi; \Phi \vdash \onet } f
    \end{align*}
    Similarly for $\zerot$.

  \item Case $\Gamma; \Phi, \phi \vdash \phi \ol\tau : \F$. The induction hypothesis gives that 
    $$\setsem{\Gamma; \Phi, \phi \vdash \tau} f = 
      \setsem{\Gamma, \psi; \Phi \vdash \tau[\phi :== \psi]} f$$
    for each $\tau$.

    \begin{align*}
         & \setsem{\Gamma; \Phi, \phi \vdash \phi \ol\tau} f \\
      = \; & (f \phi)_{\ol{\setsem{\Gamma; \Phi, \phi \vdash \tau} \rho'}} 
              \circ (\rho \phi) \ol{\setsem{\Gamma; \Phi, \phi \vdash \tau} f} \\
      = \; & (\id_{\rho \phi})_{\ol{\setsem{\Gamma; \Phi, \phi \vdash \tau} \rho'}} 
              \circ (\rho \phi) \ol{\setsem{\Gamma; \Phi, \phi \vdash \tau} f} \\
      = \; & (\rho \phi) \ol{\setsem{\Gamma; \Phi, \phi \vdash \tau} f} \\
      = \; & (\rho \psi) \ol{\setsem{\Gamma, \psi; \Phi \vdash \tau[\phi :== \psi]} f} \\
      = \; & (\id_{\rho \psi})_{\ol{\setsem{\Gamma, \psi; \Phi \vdash \tau[\phi :== \psi]} \rho'}}
              \circ (\rho \psi) \ol{\setsem{\Gamma, \psi; \Phi \vdash \tau[\phi :== \psi]} f} \\
      = \; & (f \psi)_{\ol{\setsem{\Gamma, \psi; \Phi \vdash \tau[\phi :== \psi]} \rho'}}
              \circ (\rho \psi) \ol{\setsem{\Gamma, \psi; \Phi \vdash \tau[\phi :== \psi]} f} \\
      = \; & \setsem{\Gamma, \psi; \Phi \vdash \psi \ol{\tau[\phi :== \psi]}} f \\
      = \; & \setsem{\Gamma, \psi; \Phi \vdash (\phi \ol\tau) [\phi :== \psi]} f
    \end{align*}

  \item Case $\Gamma; \Phi, \phi \vdash (\mu \phi'. \lambda \ol\alpha. H)\ol\tau : \F$. 
      The induction hypothesis gives that 
      $$\setsem{\Gamma; \Phi, \phi', \ol{\alpha}, \phi \vdash H } f
        = \setsem{\Gamma, \psi; \Phi, \phi', \ol{\alpha} \vdash H[\phi :== \psi] } f$$ 
      and 
      $$\setsem{\Gamma; \Phi, \phi \vdash \tau } f
        = \setsem{\Gamma, \psi; \Phi \vdash \tau[\phi :== \psi] } f$$ 
      for each $\tau$. 
      \begin{align*}
        & \setsem{\Gamma; \Phi, \phi \vdash (\mu \phi'. \lambda \ol\alpha. H)\ol\tau } f \\
        % = \; & (\mu \sigma^\set_f)_{\ol{\setsem{\Gamma; \Phi, \phi \vdash \tau} \rho'}}
        %         \circ (\mu T^\set_\rho) \ol{\setsem{\Gamma; \Phi, \phi \vdash \tau} f} \\
        = \; & 
           (\mu (
             \lambda F. \lambda \ol{A}. \setsem{\Gamma; \Phi, \phi', \ol{\alpha}, \phi \vdash H} f [\phi' := \id_F][\ol{\alpha := \id_A}]
           ))_{\ol{\setsem{\Gamma; \Phi, \phi \vdash \tau} \rho'}} \\
          \; & \circ
          (\mu (
            \lambda F. \lambda \ol{A}. \setsem{\Gamma; \Phi, \phi', \ol{\alpha}, \phi \vdash H} \rho[\phi' := F][\ol{\alpha := A}]
          )
        ) \ol{\setsem{ \Gamma; \Phi, \phi \vdash \tau} f} \\
        = \; & 
           (\mu (
             \lambda F. \lambda \ol{A}. \setsem{\Gamma; \Phi, \phi', \ol{\alpha}, \phi \vdash H} f [\phi' := \id_F][\ol{\alpha := \id_A}]
           ))_{\ol{\setsem{\Gamma, \psi; \Phi \vdash \tau[\phi :== \psi]} \rho'}} \\
          \; & \circ
          (\mu (
            \lambda F. \lambda \ol{A}. \setsem{\Gamma; \Phi, \phi', \ol{\alpha}, \phi \vdash H} \rho[\phi' := F][\ol{\alpha := A}]
          )
        ) \ol{\setsem{ \Gamma, \psi; \Phi \vdash \tau[\phi :== \psi]} f} \\
        = \; & 
           (\mu (
              \lambda F. \lambda \ol{A}. \setsem{\Gamma, \psi; \Phi, \phi', \ol{\alpha} \vdash H[\phi :== \psi]} f [\phi' := \id_F][\ol{\alpha := \id_A}]
           ))_{\ol{\setsem{\Gamma, \psi; \Phi \vdash \tau[\phi :== \psi]} \rho'}} \\
          \; & \circ
          (\mu (
            \lambda F. \lambda \ol{A}. \setsem{\Gamma; \Phi, \phi', \ol{\alpha}, \phi \vdash H} \rho[\phi' := F][\ol{\alpha := A}]
          )
        ) \ol{\setsem{ \Gamma, \psi; \Phi \vdash \tau[\phi :== \psi]} f} \\
        = \; & 
           (\mu (
              \lambda F. \lambda \ol{A}. \setsem{\Gamma, \psi; \Phi, \phi', \ol{\alpha} \vdash H[\phi :== \psi]} f [\phi' := \id_F][\ol{\alpha := \id_A}]
           ))_{\ol{\setsem{\Gamma, \psi; \Phi \vdash \tau[\phi :== \psi]} \rho'}} \\
          \; & \circ
          (\mu (
            \lambda F. \lambda \ol{A}. \setsem{\Gamma, \psi; \Phi, \phi', \ol{\alpha} \vdash H[\phi :== \psi]} \rho[\phi' := F][\ol{\alpha := A}]
          )
        ) \ol{\setsem{ \Gamma, \psi; \Phi \vdash \tau[\phi :== \psi]} f} \\
        % = \; & (\mu \sigma^\set_f)_{\ol{\setsem{\Gamma, \psi; \Phi \vdash \tau[\phi :== \psi]} \rho'}}
        %         \circ (\mu T^\set_\rho) \ol{\setsem{\Gamma, \psi; \Phi \vdash \tau[\phi :== \psi]} f} \\
        = \; & \setsem{\Gamma, \psi; \Phi \vdash (\mu \phi'. \lambda \ol\alpha. H[\phi :== \psi]) \ol{\tau[\phi :== \psi]} } f \\
        = \; & \setsem{\Gamma, \psi; \Phi \vdash ((\mu \phi'. \lambda \ol\alpha. H) \ol\tau)[\phi :== \psi] } f
      \end{align*} 

      \noindent
      The first and fifth equalities are by Definition~\ref{def:set-sem}.
      The third equality is by the equality of the arguments to the first $\mu$ operator:
      \begin{align*}
        & \lambda F. \lambda \ol{A}. \setsem{\Gamma; \Phi, \phi', \ol{\alpha}, \phi \vdash H} f [\phi' := \id_F][\ol{\alpha := \id_A}] \\
        & = \lambda F. \lambda \ol{A}. \setsem{\Gamma, \psi; \Phi, \phi', \ol{\alpha} \vdash H[\phi :== \psi]} f [\phi' := \id_F][\ol{\alpha := \id_A}]
      \end{align*}
      By the induction hypothesis on $H$ and the fact that the morphism $f[\phi' := \id_F][\ol{\alpha := \id_A}]
      : \rho[\phi' := F][\ol{\alpha := A}] \to \rho'[\phi' := F][\ol{\alpha := A}]$
      still satisfies the required hypotheses.
      The fourth equality is by the equality of the arguments to the second $\mu$ operator:
      \begin{align*}
        & \lambda F. \lambda \ol{A}. \setsem{\Gamma; \Phi, \phi', \ol{\alpha}, \phi \vdash H} \rho[\phi' := F][\ol{\alpha := A}] \\
        & = \lambda F. \lambda \ol{A}. \setsem{\Gamma, \psi; \Phi, \phi', \ol{\alpha} \vdash H[\phi :== \psi]} \rho[\phi' := F][\ol{\alpha := A}]
      \end{align*}

      These two functors have the same action on objects by the induction hypothesis on $H$ from Theorem~\ref{thm:demotion-objects},
      and they have the same action on morphisms by the induction hypothesis on $H$ from this theorem. 
      Thus they are the same functor with the same fixed point.

  \item Case $\Gamma; \Phi, \phi \vdash \sigma \times \tau : \F$. The induction hypothesis gives that 
      $$\setsem{\Gamma; \Phi, \phi \vdash \sigma } f
        = \setsem{\Gamma, \psi; \Phi \vdash \sigma[\phi :== \psi] } f$$ 
        and
      $$\setsem{\Gamma; \Phi, \phi \vdash \tau } f
        = \setsem{\Gamma, \psi; \Phi \vdash \tau[\phi :== \psi] } f$$ 

    \begin{align*}
           & \setsem{\Gamma; \Phi, \phi \vdash \sigma \times \tau} f \\
      = \; & \setsem{\Gamma; \Phi, \phi \vdash \sigma} f \times \setsem{\Gamma; \Phi, \phi \vdash \tau} f \\
      = \; & \setsem{\Gamma, \psi; \Phi \vdash \sigma[\phi :== \psi]} f \times \setsem{\Gamma, \psi; \Phi \vdash \tau[\phi :== \psi]} f \\
      = \; & \setsem{\Gamma, \psi; \Phi \vdash \sigma[\phi :==\psi] \times \tau[\phi :== \psi]} f \\
      = \; & \setsem{\Gamma, \psi; \Phi \vdash (\sigma \times \tau)[\phi :== \psi]} f
    \end{align*}


    The case for $\sigma + \tau$ is analogous.
\end{itemize}
\end{proof}
\end{document}

\end{itemize}


\end{proof}

\end{document}

